Some proofs on types_subset4.v

rules/types_subset4.v
@@ -1,8 +1,12 @@
 Require Import Coq.Strings.String.
 Require Import Coq.Lists.List.
+Require Import Lia.
+Require Import Coq.Logic.Decidable.
 Import ListNotations.
 
 Definition name_t := string.
+
+Definition globalname_t := string.
 
 Section type_t.
 
@@ -15,12 +19,18 @@ Section type_t.
   Inductive type_t : Type :=
     | Statement : type_t
     | Nil       : type_t
+    | Boolean   : type_t
     | Integer   : type_t
+    | Byte      : type_t
+    | Word      : type_t
+    | Real      : type_t
     | Reference : type_t -> type_t
     | OpenArray : type_t -> type_t
     | Array     : nat -> type_t -> type_t
     | Record    : list (name_t * type_t) -> type_t
-    | Procedure : list (passing_method_t * type_t) -> type_t -> type_t. 
+    | Procedure : list (passing_method_t * type_t) -> type_t -> type_t
+    | NamedRef  : globalname_t -> type_t 
+    | Abstract  : globalname_t -> type_t.
 
   Set Elimination Schemes.
 
@@ -28,12 +38,13 @@ Section type_t.
 
     Variables 
       (P : type_t -> Prop)
-      (HStatement : 
-        P Statement)
-      (HNil : 
-        P Nil)
-      (HInteger : 
-        P Integer)
+      (HStatement : P Statement)
+      (HBoolean :   P Boolean)
+      (HNil :       P Nil)
+      (HInteger :   P Integer)
+      (HByte :      P Byte)
+      (HWord :      P Word)
+      (HReal :      P Real)
       (HReference : 
         forall dtype, P dtype -> P (Reference dtype))
       (HOpenArray : 
@@ -48,14 +59,23 @@ Section type_t.
         forall args rtype, 
         (forall pass type, In (pass, type) args -> P type) -> 
         P rtype -> 
-        P (Procedure args rtype)).
+        P (Procedure args rtype))
+      (HNamedRef : 
+        forall name, P (NamedRef name))
+      (HAbstract :
+        forall name, P (Abstract name)).
 
     Fixpoint type_t_ind type : P type.
     Proof.
-      destruct type as [ | | | dtype | etype | len etype | elements | args rtype ].
+      destruct type as [ | | | | | | | dtype | etype | len etype
+                       | elements | args rtype | name | name ].
       + apply HStatement.
       + apply HNil.
+      + apply HBoolean.
       + apply HInteger.
+      + apply HByte.
+      + apply HWord.
+      + apply HReal.
       + apply HReference. apply type_t_ind.
       + apply HOpenArray. apply type_t_ind.
       + apply HArray. apply type_t_ind.
@@ -72,6 +92,8 @@ Section type_t.
           - specialize (type_t_ind (snd arg)); now subst.
           - apply IH with (1 := H).
         * apply type_t_ind.
+      + apply HNamedRef.
+      + apply HAbstract.
     Qed.
 
   End type_t_ind.
@@ -82,12 +104,18 @@ Section type_t.
     match t with
     | Statement => False
     | Nil => False
+    | Boolean => False
     | Integer => False
+    | Byte => False
+    | Word => False
+    | Real => False
     | Reference dtype => dtype = s
     | OpenArray etype => etype = s
     | Array _ etype => etype = s
     | Record elements => exists name, In (name, s) elements
     | Procedure args rtype => exists pass, In (pass, s) args \/ s = rtype
+    | NamedRef _ => False
+    | Abstract _ => False
     end.
 
   Local Fact wf_sub_type : well_founded sub_type_t.
@@ -103,17 +131,17 @@ Section type_t.
       + rewrite <- H0 in IHt. apply IHt.                (* rtype *)
   Qed.
 
-
   Section type_t_rect.
 
     Variables 
       (P : type_t -> Prop)
-      (HStatement : 
-        P Statement)
-      (HNil : 
-        P Nil)
-      (HInteger : 
-        P Integer)
+      (HStatement : P Statement)
+      (HBoolean :   P Boolean)
+      (HNil :       P Nil)
+      (HInteger :   P Integer)
+      (HByte :      P Byte)
+      (HWord :      P Word)
+      (HReal :      P Real)
       (HReference : 
         forall dtype, P dtype -> P (Reference dtype))
       (HOpenArray : 
@@ -128,15 +156,24 @@ Section type_t.
         forall args rtype, 
         (forall pass type, In (pass, type) args -> P type) -> 
         P rtype -> 
-        P (Procedure args rtype)).
+        P (Procedure args rtype))
+      (HNamedRef : 
+        forall name, P (NamedRef name))
+      (HAbstract :
+        forall name, P (Abstract name)).
 
     Theorem type_t_rect type : P type.
     Proof.
-      induction type as [ [ | | | dtype | etype | len etype | elts | args rtype ] IH ] 
+      induction type as [ [ | | | | | | | dtype | etype | len etype 
+                          | elements | args rtype | name | name ] IH ] 
           using (well_founded_induction_type wf_sub_type).
       + apply HStatement.
       + apply HNil.
+      + apply HBoolean.
       + apply HInteger.
+      + apply HByte.
+      + apply HWord.
+      + apply HReal.
       + apply HReference. apply IH. constructor.
       + apply HOpenArray. apply IH. constructor.
       + apply HArray. apply IH. constructor.
@@ -145,55 +182,197 @@ Section type_t.
       + apply HProcedure.
         - intros pass ? ?. apply IH. exists pass. left. apply H.
         - apply IH. exists ByValue. right. reflexivity.
+      + apply HNamedRef.
+      + apply HAbstract.
     Qed.
 
   End type_t_rect.
 
-
   Definition type_t_rec (P : _ -> Prop) := type_t_rect P.
 
-  Inductive TypeEqual : type_t -> type_t -> Prop :=
-    | TypeEqual_Statement : 
-        TypeEqual Statement Statement
-    | TypeEqual_Nil : 
-        TypeEqual Nil Nil
-    | TypeEqual_Integer : 
-        TypeEqual Integer Integer
-    | TypeEqual_Reference t  :  
-        TypeEqual (Reference t) (Reference t)
-    | TypeEqual_OpenArray t  :  
-        TypeEqual (OpenArray t) (OpenArray t)
-    | TypeEqual_Array len t :  
-        TypeEqual (Array len t) (Array len t)
-
-    | TypeEqual_Record elements1 elements2 : 
-        Forall2 eq (map fst elements1) (map fst elements2) -> 
-        Forall2 TypeEqual (map snd elements1) (map snd elements2) -> 
-        TypeEqual (Record elements1) (Record elements2)
-    
-    | TypeEqual_Procedure args1 rettype1 args2 rettype2 : 
-        Forall2 eq (map fst args1) (map fst args2) ->  
-        Forall2 TypeEqual (map snd args1) (map snd args2) -> 
-        TypeEqual rettype1 rettype2 ->
-        TypeEqual (Procedure args1 rettype1) (Procedure args2 rettype2)
-    .
-
-  Fact Forall2_refl X R l : 
-    (forall x : X, In x l -> R x x) -> Forall2 R l l.
-  Proof.
-    rewrite <- Forall_forall.
-    induction 1; auto.
-  Qed.
-
-
-  Fact TypeEqual_refl (t: type_t) : TypeEqual t t.
-  Proof.
-    induction t; constructor; try apply Forall2_refl.
-    + intros. reflexivity.                                 (* Record names *)
-    + intros ? ((name, type) & <- & HI)%in_map_iff. eauto. (* Record types *)
-    + intros. reflexivity.                                 (* Procedure passing *)
-    + intros ? ((pass, type) & <- & HI)%in_map_iff. eauto. (* Procedure args. *)
-    + apply IHt.                                           (* Procedure return. *)
-  Qed.
-
 End type_t.
+
+
+Module rules.
+  Variable module_t : Type.
+  Variable module_equivalent : module_t -> type_t -> type_t -> Prop.
+
+  Definition atomic_type (t: type_t) : Prop := 
+  match t with
+  | Boolean   => True
+  | Integer   => True
+  | Byte      => True
+  | Word      => True
+  | Real      => True
+  | Reference _ => True
+  | NamedRef _ => True
+  | _ => False
+  end. 
+
+  Definition structured_type (t: type_t) : Prop :=  
+  match t with
+  | OpenArray _ => True
+  | Array _ _ => True
+  | Record _ => True
+  | Procedure _ _ => True
+  | Abstract _ => True
+  | _ => False
+  end.
+
+  Definition special_type (t: type_t) : Prop :=  
+  match t with
+  | Nil => True
+  | Statement => True
+  | _ => False
+  end.
+
+  Definition reference_type (t: type_t) : Prop :=  
+  match t with
+  | Nil => True 
+  | Reference _ => True
+  | NamedRef _ => True
+  | _ => False
+  end.
+
+  Definition unsized_type (t: type_t) : Prop :=  
+  match t with
+  | OpenArray _ => True 
+  | Abstract _ => True
+  | t => special_type t
+  end.
+
+  Definition value_type (t: type_t) : Prop := atomic_type t \/ t = Nil.
+  
+  Definition return_type (t: type_t) : Prop := atomic_type t \/ t = Statement.
+  
+  Definition referenceable_type  (t: type_t) : Prop := ~(special_type t).
+
+  Definition value_parameter_type (t: type_t) : Prop := 
+    referenceable_type t \/ value_type t.
+
+
+  (* - - - - - - - - - - - - - - - - - - - - - - - - - - - - - - - - - - - - *)
+
+  Theorem atomic_and_structured_are_distinct : forall (t: type_t),
+    ~ (atomic_type t /\ structured_type t).
+  Proof.
+    intros. unfold not. intros. destruct H as [Ha Hs].
+    destruct t; simpl in *; try destruct Ha; try destruct Hs. 
+  Qed.
+
+  Theorem special_and_structured_are_distinct : forall (t: type_t),
+    ~ (special_type t /\ structured_type t).
+  Proof.
+    intros. unfold not. intros. destruct H as [Ha Hs].
+    destruct t; simpl in *; try destruct Ha; try destruct Hs. 
+  Qed.
+
+  Theorem special_and_atomic_are_distinct : forall (t: type_t),
+    ~ (special_type t /\ atomic_type t).
+  Proof.
+    intros. unfold not. intros. destruct H as [Ha Hs].
+    destruct t; simpl in *; try destruct Ha; try destruct Hs. 
+  Qed.
+
+  Theorem atomic_types_are_values : forall (t: type_t),
+    atomic_type t -> value_type t.
+  Proof.
+    intros. unfold value_type. left. apply H.
+  Qed.
+
+  Theorem return_types_are_atomic : forall (t: type_t),
+    atomic_type t -> return_type t.
+  Proof.
+    intros. unfold return_type. left. apply H.
+  Qed.
+
+  (* - - - - - - - - - - - - - - - - - - - - - - - - - - - - - - - - - - - - *)
+
+  Inductive sized_type : type_t -> Prop :=
+    | sized_type_Boolean :       sized_type Boolean
+    | sized_type_Integer :       sized_type Integer
+    | sized_type_Byte :          sized_type Byte
+    | sized_type_Word :          sized_type Word
+    | sized_type_Real :          sized_type Real
+    | sized_type_Reference t :   sized_type (Reference t)
+    | sized_type_NamedRef name : sized_type (NamedRef name)
+    | sized_type_Array len t : 
+        len > 0 -> sized_type t -> sized_type (Array len t)
+    | sized_type_Record elements : 
+        Forall sized_type (map snd elements) -> sized_type (Record elements). 
+
+  (* - - - - - - - - - - - - - - - - - - - - - - - - - - - - - - - - - - - - *)
+
+  Theorem sized_and_unsized_are_distinct : forall (t: type_t),
+    ~ (sized_type t /\ unsized_type t).
+  Proof.
+    intros. unfold not. intros.
+    destruct H as [Hs Hu].
+    inversion t; simpl in *; try destruct Hs; try destruct Hu. 
+  Qed.
+
+  Theorem sized_arrays_have_sized_elements : forall (n: nat) (t: type_t),
+    n > 0 -> sized_type (Array n t) -> sized_type t.
+  Proof.
+    intros n t H.
+    intros. inversion H0. apply H4.
+  Qed.
+
+  Theorem sized_records_have_sized_elements : 
+    forall (elements: list (name_t * type_t)),
+    sized_type (Record elements) -> Forall sized_type (map snd elements).
+  Proof.
+    intros.
+    inversion H. apply H1.
+  Qed.
+
+  Theorem sized_types_are_referenceable : forall (t: type_t),
+    sized_type t -> referenceable_type t.    
+  Proof.
+    intros. inversion H; subst; unfold referenceable_type; auto.
+  Qed.
+
+
+(* - - - - - - - - - - - - - - - - - - - - - - - - - - - - - - - - - - - - - *)
+(* Type Validity *)
+(* - - - - - - - - - - - - - - - - - - - - - - - - - - - - - - - - - - - - - *)
+
+Inductive valid_type : type_t -> Prop :=
+  | valid_type_Statement : valid_type Statement
+  | valid_type_Nil :       valid_type Nil
+  | valid_type_Boolean :   valid_type Boolean
+  | valid_type_Integer :   valid_type Integer
+  | valid_type_Byte :      valid_type Byte
+  | valid_type_Word :      valid_type Word
+  | valid_type_Real :      valid_type Real
+  | valid_type_Reference t : 
+      sized_type t -> 
+      valid_type t -> 
+      valid_type (Reference t)
+  | valid_type_OpenArray t : 
+      valid_type t -> 
+      sized_type t -> 
+      valid_type (OpenArray t)
+  | valid_type_Array len t : 
+      len > 0 -> 
+      valid_type t -> 
+      sized_type t -> 
+      valid_type (Array len t)
+  | valid_type_Record elements :
+      NoDup (map fst elements) ->
+      Forall sized_type (map snd elements) -> 
+      Forall valid_type (map snd elements) -> 
+      valid_type (Record elements) 
+  | valid_type_Procedure args rettype : 
+      valid_type rettype -> 
+      return_type rettype ->
+      Forall valid_type (map snd args) -> 
+      Forall (fun a => fst a = ByValue -> value_parameter_type (snd a)) args ->
+      Forall (fun a => fst a = ByReference -> reference_type (snd a)) args ->
+      valid_type (Procedure args rettype)
+  | valid_type_NamedRef name : 
+      valid_type (NamedRef name)    (* XXX *) 
+  | valid_type_Abstract name : 
+      valid_type (Abstract name).   (* XXX *)
+
+End rules.
